

# Proof of the Euclidean Algorithm

## Contents

<b>1</b>	<b>Number Theory</b>	<b>2</b>
1.1	Euclidean Algorithm . . . . .	2
1.2	Divisibility Sets . . . . .	2
1.3	Corollary: Divisibility of $r$ . . . . .	2

# 1 Number Theory

## 1.1 Euclidean Algorithm

**Theorem 1.1** (Euclidean Algorithm). *Let  $a$  and  $b$  be integers with  $b \neq 0$ . Then there exist integers  $q$  and  $r$  such that*

$$a = bq + r, \quad \text{where } r = (a \bmod b) \text{ and } 0 \leq r < |b|.$$

*and greatest common divisor,  $\gcd(a, b)$ , of  $a$  and  $b$  satisfies*

$$\gcd(a, b) = \gcd(b, r).$$

## 1.2 Divisibility Sets

**Definition 1.2.** *For integers  $a$  and  $b$ , not both zero, define*

$$D(a, b) = \{d \in \mathbb{Z} : d \mid a \text{ and } d \mid b\}.$$

*The  $\gcd(a, b)$  of  $a$  and  $b$  is*

$$\max(D(a, b)).$$

## 1.3 Corollary: Divisibility of $r$

**Corollary 1.3.** *Given  $a$ ,  $b$ , and  $r$  as in Theorem 1.1, if  $d \mid a$  and  $d \mid b$ , then  $d \mid r$ .*

*Proof.* Since  $d \mid a$  and  $d \mid b$ , we can write  $a = nd$  and  $b = md$  for some integers  $n, m$ . Then, by the division relation  $a = bq + r$ , we have

$$r = a - bq = nd - (md)q = d(n - mq),$$

so  $d \mid r$ . □

*Proof.* From Corollary 1.3, this means

$$\forall d \in D(a, b), \text{ since } d \mid a \text{ and } d \mid b, d \mid r.$$

Hence, with  $d \mid b$  and  $d \mid r$ , by using Definition 1.2, we know that  $d \in D(b, r)$ .

It follows that, for the integers  $a$  and  $b$  under consideration,

$$\forall d \in D(a, b), d \in D(b, r),$$

meaning

$$D(a, b) \subseteq D(b, r).$$

Using an identical argument applied to integers  $b$  and  $r$ , we have

$$\forall d \in D(b, r), d \mid b, \text{ and } d \mid r, \text{ so } d \mid a,$$

and so,

$$\forall d \in D(b, r), d \in D(a, b),$$

meaning

$$D(b, r) \subseteq D(a, b).$$

As both  $D(b, r) \subseteq D(a, b)$  and  $D(a, b) \subseteq D(b, r)$ , we conclude that

$$D(a, b) = D(b, r).$$

Since  $D(a, b) = D(b, r)$ , it follows that

$$\max D(a, b) = \max D(b, r).$$

Moreover, by Definition 1.2,

$$\gcd(a, b) = \max D(a, b) \quad \text{and} \quad \gcd(b, r) = \max D(b, r).$$

Therefore,

$$\boxed{\gcd(a, b) = \gcd(b, r)}.$$

□